src/sequential/DelayedStep.v
@@ -1,0 +1,221 @@
+Require Import RelationClasses.
+Require Import Program.
+
+From sflib Require Import sflib.
+From Paco Require Import paco.
+
+From PromisingLib Require Import Axioms.
+From PromisingLib Require Import Basic.
+From PromisingLib Require Import Loc.
+From PromisingLib Require Import DenseOrder.
+From PromisingLib Require Import Language.
+
+Require Import Event.
+Require Import Time.
+Require Import View.
+Require Import Cell.
+Require Import Memory.
+Require Import MemoryFacts.
+Require Import TView.
+Require Import Local.
+Require Import Thread.
+Require Import Configuration.
+
+Require Import PromiseConsistent.
+Require Import Cover.
+Require Import MemorySplit.
+Require Import MemoryMerge.
+Require Import FulfillStep.
+Require Import Pred.
+Require Import Trace.
+Require Import MemoryProps.
+Require Import LowerMemory.
+Require Import FulfillStep.
+Require Import ReorderStepPromise.
+Require Import Pred.
+Require Import Trace.
+
+Require Import SeqLib.
+Require Import gSimAux.
+Require Import Delayed.
+
+Set Implicit Arguments.
+Set Nested Proofs Allowed.
+
+
+Section DStep.
+  Variable lang: language.
+
+  Variant delayed_step (e: ThreadEvent.t) (e1 e4: Thread.t lang): Prop :=
+  | delayed_step_intro
+      e2 e3 pf
+      (PROMISES: rtc (tau (@pred_step is_promise _)) e1 e2)
+      (LOWERS: rtc (tau lower_step) e2 e3)
+      (STEP_RELEASE: Thread.step pf e e3 e4)
+      (EVENT_RELEASE: release_event e)
+  .
+
+  Variant delayed_steps: forall (e: MachineEvent.t) (e1 e2: Thread.t lang), Prop :=
+  | delayed_steps_promises
+      e1 e2 e3
+      (DSTEPS: rtc (tau delayed_step) e1 e2)
+      (PROMISES: rtc (tau (@pred_step is_promise _)) e2 e3):
+    delayed_steps MachineEvent.silent e1 e3
+  | delayed_steps_step
+      e te e1 e2 e3
+      (DSTEPS: rtc (tau (@pred_step is_promise _)) e1 e2)
+      (DSTEP: delayed_step te e2 e3)
+      (EVENT: e = ThreadEvent.get_machine_event te):
+    delayed_steps e e1 e3
+  .
+
+  Definition delayed_consistent (e1: Thread.t lang): Prop :=
+    forall mem1 (CAP: Memory.cap e1.(Thread.memory) mem1),
+    exists e e2,
+      (<<DSTEPS: delayed_steps
+                   e (Thread.mk _ (Thread.state e1) (Thread.local e1) (Thread.sc e1) mem1) e2>>) /\
+      ((<<FAILURE: e = MachineEvent.failure>>) \/
+       (<<SILENT: e = MachineEvent.silent>>) /\
+         (<<PROMISES: Local.promises (Thread.local e2) = Memory.bot>>)).
+
+  Variant non_release_step (e: ThreadEvent.t) (e1 e2: Thread.t lang): Prop :=
+  | non_release_step_intro
+      pf
+      (STEP: Thread.step pf e e1 e2)
+      (RELEASE: ~ release_event e)
+  .
+
+  Variant non_release_plus_step (e: ThreadEvent.t) (e1 e3: Thread.t lang): Prop :=
+  | non_release_plus_step_intro
+      e2 pf
+      (STEPS: rtc (tau non_release_step) e1 e2)
+      (STEP: Thread.step pf e e2 e3)
+      (RELEASE: release_event e)
+  .
+
+  Variant steps: forall (e: MachineEvent.t) (e1 e2: Thread.t lang), Prop :=
+  | steps_non_release
+      e1 e2 e3
+      (STEPS: rtc (tau non_release_plus_step) e1 e2)
+      (NSTEPS: rtc (tau non_release_step) e2 e3):
+    steps MachineEvent.silent e1 e3
+  | steps_release
+      e e1 e2 e3
+      (STEPS: rtc (tau non_release_plus_step) e1 e2)
+      (STEP: non_release_plus_step e e2 e3):
+    steps (ThreadEvent.get_machine_event e) e1 e3
+  .
+
+  Lemma non_release_silent
+        e
+        (RELEASE: ~ release_event e):
+    ThreadEvent.get_machine_event e = MachineEvent.silent.
+  Proof.
+    destruct e; ss.
+  Qed.
+
+  Lemma plus_step_steps
+        pf e e1 e2 e3
+        (STEPS: rtc (@Thread.tau_step _) e1 e2)
+        (STEP: Thread.step pf e e2 e3):
+    steps (ThreadEvent.get_machine_event e) e1 e3.
+  Proof.
+    induction STEPS; i.
+    { destruct (classic (release_event e)).
+      - econs 2; try refl. econs; try refl; eauto.
+      - rewrite non_release_silent; eauto.
+        econs 1; try refl. econs 2; try refl.
+        econs; try eapply non_release_silent; eauto.
+        econs; eauto.
+    }
+    exploit IHSTEPS; eauto. i. clear IHSTEPS.
+    clear - H x0.
+    inv H. inv TSTEP.
+    destruct (classic (release_event e0)).
+    { inv x0.
+      { econs 1; try exact NSTEPS.
+        econs 2; try exact STEPS.
+        econs; try exact EVENT.
+        econs; try refl; eauto.
+      }
+      { econs 2; try exact STEP0.
+        econs 2; try exact STEPS.
+        econs; try exact EVENT.
+        econs; try refl; eauto.
+      }
+    }
+    { inv x0.
+      { inv STEPS.
+        { econs 1; [refl|].
+          econs 2; try exact NSTEPS.
+          econs; try exact EVENT.
+          econs; eauto.
+        }
+        { econs 1; try exact NSTEPS.
+          econs 2; try exact H2.
+          inv H0. econs; try exact EVENT0.
+          inv TSTEP. econs; try exact STEP0; ss.
+          econs 2; try exact STEPS.
+          econs; try exact EVENT. econs; eauto.
+        }
+      }
+      { inv STEPS.
+        { econs 2; [refl|].
+          inv STEP0. econs; try exact STEP1; ss.
+          econs 2; try exact STEPS.
+          econs; try exact EVENT.
+          econs; eauto.
+        }
+        { econs 2; try exact STEP0.
+          econs 2; try exact H2.
+          inv H0. econs; try exact EVENT0.
+          inv TSTEP. econs; try exact STEP1; ss.
+          econs 2; try exact STEPS.
+          econs; try exact EVENT.
+          econs; eauto.
+        }
+      }
+    }
+  Qed.
+
+  Variant delayed_thread fin (e_src e_tgt: Thread.t lang): Prop :=
+    | delayed_thread_intro
+        lc_lower
+        (LOWER_LC: lower_local lc_lower (Thread.local e_tgt))
+        (LOWER_SC: TimeMap.le (Thread.sc e_src) (Thread.sc e_tgt))
+        (LOWER_MEM: lower_memory (Thread.memory e_src) (Thread.memory e_tgt))
+        (DELAYED: delayed (Thread.state e_src) (Thread.state e_tgt)
+                          (Thread.local e_src) lc_lower
+                          (Thread.sc e_src) (Thread.memory e_src) fin)
+  .
+
+  Definition committed_thread (e1 e2: Thread.t lang) :=
+    committed (Thread.memory e1) (Local.promises (Thread.local e1))
+              (Thread.memory e2) (Local.promises (Thread.local e2)).
+
+  Lemma non_release_step_delayed
+        e1_src
+        fin e_tgt e1_tgt e2_tgt
+        (DELAYED: delayed_thread fin e1_src e1_tgt)
+        (STEP: non_release_step e_tgt e1_tgt e2_tgt)
+        (CONS: Local.promise_consistent (Thread.local e2_tgt)):
+    exists e2_src,
+      (<<PROMISES: rtc (tau (@pred_step is_promise _)) e1_src e2_src>>) /\
+        (<<DELAYED: delayed_thread (fin \4/ committed_thread e1_src e2_src) e2_src e2_tgt>>).
+  Proof.
+  Admitted.
+End DStep.
+
+Module DConfiguration.
+  Variant step: forall (e: MachineEvent.t) (tid: Ident.t) (c1 c2: Configuration.t), Prop :=
+  | step_intro
+      e tid c1 lang st1 lc1 st2 lc2 sc2 mem2
+      (TID: IdentMap.find tid (Configuration.threads c1) = Some (existT _ lang st1, lc1))
+      (DSTEPS: delayed_steps e (Thread.mk _ st1 lc1 (Configuration.sc c1) (Configuration.memory c1))
+                             (Thread.mk _ st2 lc2 sc2 mem2))
+      (CONSISTENT: e <> MachineEvent.failure ->
+                   delayed_consistent (Thread.mk _ st2 lc2 sc2 mem2)):
+      step e tid c1
+           (Configuration.mk (IdentMap.add tid (existT _ _ st2, lc2) (Configuration.threads c1)) sc2 mem2)
+  .
+End DConfiguration.
